## Solution1
``` java
class Solution {
    public int subarraySum(int[] nums, int k) {
        Map<Integer, Integer> map = new HashMap<>();
        int count = 0;
        int sum = 0;
        map.put(0, 1);
        
        for (int num : nums) {
            sum += num;
            if (map.containsKey(sum - k)) {
                count += map.get(sum - k);
            }
            map.put(sum, map.getOrDefault(sum, 0) + 1);
        }
        return count;
    }
}
```

## note 
* The idea is to store the previously calculated Sum[0, i] and its frequency into a hashmap. Once we can find 
Sum[0, j] - Sum[0, i] = k, we increment the count by the frequency of Sum[0, 1] which we have stored earlier.
* Remember to initialize the hashmap with (0, 1) stored so that we could get our first subarray sum from.
